wip

src/lib/Coquill/Array.v
@@ -1,7 +1,9 @@
 Set Default Goal Selector "!". 
 
 From Coq Require Import NArith.
+
 From Coquill Require Import List.
+From Coquill Require HalfOpenRange.
 
 Open Scope N_scope.
 
@@ -12,13 +14,35 @@ Record t (A : Type) (n : N) : Type := make {
   length_spec : length inner_list = n;
 }.
 
+Arguments make {A n} inner_list length_spec.
+Arguments inner_list {A n} _.
+Arguments length_spec {A n} _.
+
 Hint Constructors t : array.
 
-Definition empty (A : Type) : t A 0 := make A 0 [] eq_refl.
+Definition empty (A : Type) : t A 0 := make [] eq_refl.
 
 Program Definition repeat {A : Type} (x : A) (n : N) : t A n :=
-  make A n (List.repeat x n) _.
+  make (List.repeat x n) _.
 Next Obligation.
 Proof.
   apply repeat_length.
 Qed.
+
+Section UpdateRange.
+  Context {A : Type}.
+  Context {n : N}.
+
+  Program Definition update_range (arr : t A n) (r : HalfOpenRange.t) (x : A) (upper_spec : HalfOpenRange.upper r <= n) : t A n :=
+    make (List.update_range (inner_list arr) r x _) _.
+  Next Obligation.
+  Proof.
+    rewrite length_spec.
+    auto.
+  Qed.
+  Next Obligation.
+  Proof.
+    rewrite length_update_range.
+    apply length_spec.
+  Qed. 
+End UpdateRange.
